Impl/MarshallingImpl.i.dfy
@@ -529,7 +529,6 @@ module MarshallingImpl {
   method {:fuel SizeOfV,4} nodeToVal(shared node: Node)
   returns (v : V, size: uint64)
   requires node.Inv()
-  requires SSM.WFNode(node.I())
   requires BT.WFNode(node.I())
   requires BucketsLib.BucketListWellMarshalled(BucketImpl.MutBucket.ILseq(node.buckets))
   ensures ValidVal(v)
@@ -590,7 +589,6 @@ module MarshallingImpl {
   requires SSI.WFSector(sector)
   requires SSM.WFSector(SSI.ISector(sector))
   requires sector.SectorNode?
-  requires sector.SectorNode? ==> SSM.WFNode(sector.node.I())
   requires sector.SectorNode? ==> BT.WFNode(sector.node.I())
   requires sector.SectorNode? ==> 
     BucketsLib.BucketListWellMarshalled(BucketImpl.MutBucket.ILseq(sector.node.buckets))
@@ -634,7 +632,6 @@ module MarshallingImpl {
   ensures s.lSome? ==> SSI.WFSector(s.value)
   ensures s.lSome? ==> SSM.WFSector(SSI.ISector(s.value))
   ensures ISectorOpt(s.Option()) == IMM.parseSector(data[start..])
-  ensures s.lSome? && s.value.SectorNode? ==> SSM.WFNode(s.value.node.I())
   ensures s.lSome? && s.value.SectorNode? ==> BT.WFNode(s.value.node.I())
   {
     IMM.reveal_parseSector();
@@ -673,7 +670,6 @@ module MarshallingImpl {
   ensures s.lSome? ==> SSI.WFSector(s.value)
   ensures s.lSome? ==> SSM.WFSector(SSI.ISector(s.value))
   ensures ISectorOpt(s.Option()) == IMM.parseCheckedSector(data)
-  ensures s.lSome? && s.value.SectorNode? ==> SSM.WFNode(s.value.node.I())
   ensures s.lSome? && s.value.SectorNode? ==> BT.WFNode(s.value.node.I())
   {
     if |data| as uint64 >= 32 {
@@ -758,8 +754,6 @@ module MarshallingImpl {
   method MarshallCheckedSector(shared sector: Sector) returns (data : array?<byte>)
   requires SSI.WFSector(sector)
   requires SSM.WFSector(SSI.ISector(sector))
-  requires sector.SectorNode? ==> SSM.WFNode(sector.node.I())
-  requires sector.SectorNode? ==> BT.WFNode(sector.node.I())
   requires sector.SectorSuperblock? ==> JC.WFSuperblock(sector.superblock)
   ensures sector.SectorIndirectionTable? ==> 
     sector.indirectionTable.Inv()
