Impl/Mkfs.i.dfy
@@ -45,7 +45,7 @@ module MkfsImpl {
 
     linear var node := Node.EmptyNode();
     ghost var i:SSM.Sector := SSI.ISector(SSI.SectorNode(node));
-    assert SSM.WFNode(i.node) by {
+    assert BT.WFNode(i.node) by {
       reveal_WeightBucketList();
     }
 
